Factor out the shallow interface

theories/Shallow.v
@@ -36,13 +36,24 @@ From Coq Require Import
 From stdpp Require Import
   base gmap.
 From Em Require Import
-  Prelude Spec.
+  Prelude
+  Shallow.Interface
+  Spec.
 
 #[local] Set Implicit Arguments.
 
-Class MFail (M : Type → Type) : Type :=
-  fail : ∀ A, M A.
-#[global] Arguments fail {M _ A}.
+(* This module implements type inference for STLC
+   using a shallow representation of constraints.
+   Essentially, constraints are nothing more than propositions in Coq.
+   This results in a fairly straightforward implementation,
+   but one which is essentially unusable, because we cannot inspect
+   the witnesses for these propositions. This is problematic,
+   because these witnesses are the unified type variables
+   which give the type and the elaboration of the term. *)
+
+(* Monadic type inference for STLC is expressed as a computation inside TypeCheckM.
+   Note that STLC requires unification of type variables.
+   These type variables are introduced by the exists_ty computation *)
 
 Fixpoint check (Γ : Env) (e : Exp) (t : Ty) : Prop :=
   match e with
@@ -81,123 +92,6 @@ Definition example_cki : Exp :=
 
 Compute exists t, check empty example_not t.
 Compute exists t, check empty example_cki t.
-
-(* This module implements type inference for STLC
-   using a shallow representation of constraints.
-   Essentially, constraints are nothing more than propositions in Coq.
-   This results in a fairly straightforward implementation,
-   but one which is essentially unusable, because we cannot inspect
-   the witnesses for these propositions. This is problematic,
-   because these witnesses are the unified type variables
-   which give the type and the elaboration of the term. *)
-
-(* Monadic type inference for STLC is expressed as a computation inside TypeCheckM.
-   Note that STLC requires unification of type variables.
-   These type variables are introduced by the exists_ty computation *)
-
-Class TypeCheckM (M : Type -> Type) {mretM : MRet M} {mbindM : MBind M} {mfailM : MFail M} : Type :=
-  MkTcM
-    { equals (t1 t2 : Ty) : M unit;
-      pick : M Ty;
-    }.
-#[global] Arguments TypeCheckM M {_ _ _}.
-
-Class WeakestPre (M : Type -> Type) : Type :=
-  WP [A] : M A -> (A -> Prop) -> Prop.
-Class WeakestLiberalPre (M : Type -> Type) : Type :=
-  WLP [A] : M A -> (A -> Prop) -> Prop.
-
-Class AxiomaticSemantics
-  (M : Type -> Type) {mretM : MRet M} {mbindM : MBind M} {mfailM : MFail M}
-  {tcmM : TypeCheckM M} {wpM : WeakestPre M} {wlpM : WeakestLiberalPre M} : Type :=
-  { (* WP / Total correctness *)
-    ax_wp_ret {A} (a : A) (Q : A -> Prop) :
-      WP (mret a) Q <-> Q a;
-    ax_wp_bind {A B} (f : A -> M B) (m : M A) (Q : B -> Prop) :
-      WP (mbind f m) Q <-> WP m (fun a => WP (f a) Q);
-    ax_wp_fail {A} (Q : A -> Prop) :
-      WP fail Q <-> False;
-    ax_wp_equals (t1 t2 : Ty) (Q : unit -> Prop) :
-      WP (equals t1 t2) Q <-> t1 = t2 /\ Q tt;
-    ax_wp_pick (Q : Ty -> Prop) :
-      WP pick Q <-> exists t, Q t;
-    ax_wp_mono {A} (P Q : A -> Prop) (m : M A) :
-      (forall a, P a -> Q a) -> WP m P -> WP m Q;
-
-    (* WLP / Partial correctness *)
-    ax_wlp_ret {A} (a : A) (Q : A -> Prop) :
-      WLP (mret a) Q <-> Q a ;
-    ax_wlp_bind {A B} (f : A -> M B) (m : M A) (Q : B -> Prop) :
-      WLP (mbind f m) Q <-> WLP m (fun a => WLP (f a) Q);
-    ax_wlp_fail {A} (Q : A -> Prop) :
-      WLP fail Q <-> True;
-    ax_wlp_equals (t1 t2 : Ty) (Q : unit -> Prop) :
-      WLP (equals t1 t2) Q <-> (t1 = t2 -> Q tt);
-    ax_wlp_pick (Q : Ty -> Prop) :
-      WLP pick Q <-> forall t, Q t;
-    ax_wlp_mono {A} (P Q : A -> Prop) (m : M A) :
-      (forall a, P a -> Q a) -> WLP m P -> WLP m Q;
-
-    ax_wp_impl_wlp {A} (m : M A) (P : A -> Prop) (Q : Prop) :
-      (WP m P -> Q) <-> WLP m (fun a => P a -> Q);
-  }.
-#[global] Arguments AxiomaticSemantics M {_ _ _ _ _ _}.
-
-Class TypeCheckLogicM
-  M {mretM : MRet M} {bindM : MBind M} {failM : MFail M} {tcM : TypeCheckM M}
-    {wpM : WeakestPre M} {wlpM : WeakestLiberalPre M} : Type :=
-
-  { wp_pure [A] (a : A) (Q : A -> Prop) :
-      Q a -> WP (mret a) Q;
-    wp_bind [A B] (m : M A) (f : A -> M B) (Q : B -> Prop) :
-      WP m (fun a => WP (f a) Q) -> WP (mbind f m) Q;
-    wp_equals (σ τ : Ty) (Q : unit -> Prop) :
-      σ = τ /\ Q tt -> WP (equals σ τ) Q;
-    wp_pick [Q : Ty -> Prop] (τ : Ty) :
-      (forall τ', τ = τ' -> Q τ') -> WP pick Q;
-    wp_fail [A] (Q : A -> Prop) :
-      False -> WP fail Q;
-    wp_mono [A] (m : M A) (P Q : A -> Prop) :
-      (forall a, P a -> Q a) -> (WP m P -> WP m Q);
-
-    wlp_pure [A] (a : A) (Q : A -> Prop) :
-      Q a -> WLP (mret a) Q;
-    wlp_bind [A B] (m : M A) (f : A -> M B) (Q : B -> Prop) :
-      WLP m (fun a => WLP (f a) Q) -> WLP (mbind f m) Q;
-    wlp_equals (σ τ : Ty) (Q : unit -> Prop) :
-      (σ = τ -> Q tt) -> WLP (equals σ τ) Q;
-    wlp_pick (Q : Ty -> Prop) :
-      (forall τ, Q τ) -> WLP pick Q;
-    wlp_fail [A] (Q : A -> Prop) :
-      True -> WLP fail Q;
-    wlp_mono [A] (m : M A) (P Q : A -> Prop) :
-      (forall a, P a -> Q a) ->
-      (WLP m P -> WLP m Q);
-
-    wp_impl [A] (m : M A) (P : A -> Prop) (Q : Prop) :
-      WLP m (fun a1 => P a1 -> Q) -> (WP m P -> Q);
-
-  }.
-#[global] Arguments TypeCheckLogicM _ {_ _ _ _ _ _}.
-
-#[export] Instance axiomatic_tcmlogic `{AxiomaticSemantics M} :
-  TypeCheckLogicM M.
-Proof.
-  constructor; intros *.
-  - now rewrite ax_wp_ret.
-  - now rewrite ax_wp_bind.
-  - now rewrite ax_wp_equals.
-  - rewrite ax_wp_pick. exists τ. auto.
-  - now rewrite ax_wp_fail.
-  - apply ax_wp_mono.
-  - now rewrite ax_wlp_ret.
-  - now rewrite ax_wlp_bind.
-  - now rewrite ax_wlp_equals.
-  - now rewrite ax_wlp_pick.
-  - now rewrite ax_wlp_fail.
-  - apply ax_wlp_mono.
-  - now rewrite ax_wp_impl_wlp.
-Qed.
 
 (* #[local] Notation "x <- ma ;; mb" := (bind ma (fun x => mb)) *)
 (*   (at level 80, ma at next level, mb at level 200, right associativity). *)
