theories/Shallow/Interface.v
@@ -1,0 +1,149 @@
+(******************************************************************************)
+(* Copyright (c) 2023 Denis Carnier, Steven Keuchel                           *)
+(* All rights reserved.                                                       *)
+(*                                                                            *)
+(* Redistribution and use in source and binary forms, with or without         *)
+(* modification, are permitted provided that the following conditions are     *)
+(* met:                                                                       *)
+(*                                                                            *)
+(* 1. Redistributions of source code must retain the above copyright notice,  *)
+(*    this list of conditions and the following disclaimer.                   *)
+(*                                                                            *)
+(* 2. Redistributions in binary form must reproduce the above copyright       *)
+(*    notice, this list of conditions and the following disclaimer in the     *)
+(*    documentation and/or other materials provided with the distribution.    *)
+(*                                                                            *)
+(* THIS SOFTWARE IS PROVIDED BY THE COPYRIGHT HOLDERS AND CONTRIBUTORS        *)
+(* "AS IS" AND ANY EXPRESS OR IMPLIED WARRANTIES, INCLUDING, BUT NOT LIMITED  *)
+(* TO, THE IMPLIED WARRANTIES OF MERCHANTABILITY AND FITNESS FOR A PARTICULAR *)
+(* PURPOSE ARE DISCLAIMED. IN NO EVENT SHALL THE COPYRIGHT HOLDER OR          *)
+(* CONTRIBUTORS BE LIABLE FOR ANY DIRECT, INDIRECT, INCIDENTAL, SPECIAL,      *)
+(* EXEMPLARY, OR CONSEQUENTIAL DAMAGES (INCLUDING, BUT NOT LIMITED TO,        *)
+(* PROCUREMENT OF SUBSTITUTE GOODS OR SERVICES; LOSS OF USE, DATA, OR         *)
+(* PROFITS; OR BUSINESS INTERRUPTION) HOWEVER CAUSED AND ON ANY THEORY OF     *)
+(* LIABILITY, WHETHER IN CONTRACT, STRICT LIABILITY, OR TORT (INCLUDING       *)
+(* NEGLIGENCE OR OTHERWISE) ARISING IN ANY WAY OUT OF THE USE OF THIS         *)
+(* SOFTWARE, EVEN IF ADVISED OF THE POSSIBILITY OF SUCH DAMAGE.               *)
+(******************************************************************************)
+
+From Coq Require Import
+  Classes.Morphisms_Prop
+(*   Lists.List *)
+  Program.Tactics
+  Strings.String.
+(* From Equations Require Import *)
+(*   Equations. *)
+From stdpp Require Import
+  base gmap.
+From Em Require Import
+  Prelude Spec.
+
+#[local] Set Implicit Arguments.
+
+Class MFail (M : Type → Type) : Type :=
+  fail : ∀ A, M A.
+#[global] Arguments fail {M _ A}.
+
+Class TypeCheckM (M : Type -> Type) {mretM : MRet M} {mbindM : MBind M} {mfailM : MFail M} : Type :=
+  MkTcM
+    { equals (t1 t2 : Ty) : M unit;
+      pick : M Ty;
+    }.
+#[global] Arguments TypeCheckM M {_ _ _}.
+
+Class WeakestPre (M : Type -> Type) : Type :=
+  WP [A] : M A -> (A -> Prop) -> Prop.
+Class WeakestLiberalPre (M : Type -> Type) : Type :=
+  WLP [A] : M A -> (A -> Prop) -> Prop.
+
+Class AxiomaticSemantics
+  (M : Type -> Type) {mretM : MRet M} {mbindM : MBind M} {mfailM : MFail M}
+  {tcmM : TypeCheckM M} {wpM : WeakestPre M} {wlpM : WeakestLiberalPre M} : Type :=
+  { (* WP / Total correctness *)
+    ax_wp_ret {A} (a : A) (Q : A -> Prop) :
+      WP (mret a) Q <-> Q a;
+    ax_wp_bind {A B} (f : A -> M B) (m : M A) (Q : B -> Prop) :
+      WP (mbind f m) Q <-> WP m (fun a => WP (f a) Q);
+    ax_wp_fail {A} (Q : A -> Prop) :
+      WP fail Q <-> False;
+    ax_wp_equals (t1 t2 : Ty) (Q : unit -> Prop) :
+      WP (equals t1 t2) Q <-> t1 = t2 /\ Q tt;
+    ax_wp_pick (Q : Ty -> Prop) :
+      WP pick Q <-> exists t, Q t;
+    ax_wp_mono {A} (P Q : A -> Prop) (m : M A) :
+      (forall a, P a -> Q a) -> WP m P -> WP m Q;
+
+    (* WLP / Partial correctness *)
+    ax_wlp_ret {A} (a : A) (Q : A -> Prop) :
+      WLP (mret a) Q <-> Q a ;
+    ax_wlp_bind {A B} (f : A -> M B) (m : M A) (Q : B -> Prop) :
+      WLP (mbind f m) Q <-> WLP m (fun a => WLP (f a) Q);
+    ax_wlp_fail {A} (Q : A -> Prop) :
+      WLP fail Q <-> True;
+    ax_wlp_equals (t1 t2 : Ty) (Q : unit -> Prop) :
+      WLP (equals t1 t2) Q <-> (t1 = t2 -> Q tt);
+    ax_wlp_pick (Q : Ty -> Prop) :
+      WLP pick Q <-> forall t, Q t;
+    ax_wlp_mono {A} (P Q : A -> Prop) (m : M A) :
+      (forall a, P a -> Q a) -> WLP m P -> WLP m Q;
+
+    ax_wp_impl_wlp {A} (m : M A) (P : A -> Prop) (Q : Prop) :
+      (WP m P -> Q) <-> WLP m (fun a => P a -> Q);
+  }.
+#[global] Arguments AxiomaticSemantics M {_ _ _ _ _ _}.
+
+Class TypeCheckLogicM
+  M {mretM : MRet M} {bindM : MBind M} {failM : MFail M} {tcM : TypeCheckM M}
+    {wpM : WeakestPre M} {wlpM : WeakestLiberalPre M} : Type :=
+
+  { wp_pure [A] (a : A) (Q : A -> Prop) :
+      Q a -> WP (mret a) Q;
+    wp_bind [A B] (m : M A) (f : A -> M B) (Q : B -> Prop) :
+      WP m (fun a => WP (f a) Q) -> WP (mbind f m) Q;
+    wp_equals (σ τ : Ty) (Q : unit -> Prop) :
+      σ = τ /\ Q tt -> WP (equals σ τ) Q;
+    wp_pick [Q : Ty -> Prop] (τ : Ty) :
+      (forall τ', τ = τ' -> Q τ') -> WP pick Q;
+    wp_fail [A] (Q : A -> Prop) :
+      False -> WP fail Q;
+    wp_mono [A] (m : M A) (P Q : A -> Prop) :
+      (forall a, P a -> Q a) -> (WP m P -> WP m Q);
+
+    wlp_pure [A] (a : A) (Q : A -> Prop) :
+      Q a -> WLP (mret a) Q;
+    wlp_bind [A B] (m : M A) (f : A -> M B) (Q : B -> Prop) :
+      WLP m (fun a => WLP (f a) Q) -> WLP (mbind f m) Q;
+    wlp_equals (σ τ : Ty) (Q : unit -> Prop) :
+      (σ = τ -> Q tt) -> WLP (equals σ τ) Q;
+    wlp_pick (Q : Ty -> Prop) :
+      (forall τ, Q τ) -> WLP pick Q;
+    wlp_fail [A] (Q : A -> Prop) :
+      True -> WLP fail Q;
+    wlp_mono [A] (m : M A) (P Q : A -> Prop) :
+      (forall a, P a -> Q a) ->
+      (WLP m P -> WLP m Q);
+
+    wp_impl [A] (m : M A) (P : A -> Prop) (Q : Prop) :
+      WLP m (fun a1 => P a1 -> Q) -> (WP m P -> Q);
+
+  }.
+#[global] Arguments TypeCheckLogicM _ {_ _ _ _ _ _}.
+
+#[export] Instance axiomatic_tcmlogic `{AxiomaticSemantics M} :
+  TypeCheckLogicM M.
+Proof.
+  constructor; intros *.
+  - now rewrite ax_wp_ret.
+  - now rewrite ax_wp_bind.
+  - now rewrite ax_wp_equals.
+  - rewrite ax_wp_pick. exists τ. auto.
+  - now rewrite ax_wp_fail.
+  - apply ax_wp_mono.
+  - now rewrite ax_wlp_ret.
+  - now rewrite ax_wlp_bind.
+  - now rewrite ax_wlp_equals.
+  - now rewrite ax_wlp_pick.
+  - now rewrite ax_wlp_fail.
+  - apply ax_wlp_mono.
+  - now rewrite ax_wp_impl_wlp.
+Qed.
